TODO: A, B, C, D, x, differentiation on x.

> **Definition \[inner-corner-deriv\].** For any cap \\(K\\), \\(\mathbf{v}_K^+ (t)\\) is the right derivative of \\(\mathbf{x}\\) at \\(t\\) and \\(\mathbf{v}_K^- (t)\\) is the left derivative of \\(\mathbf{x}\\) at \\(t\\). ^def-inner-corner-deriv
> \\[
> \mathbf{v}_K^{-} (t_0) = \lim_{t \rightarrow t_0^-} \frac{\mathbf{x}(t) - \mathbf{x}(t_0)}{t - t_0} \qquad
> \mathbf{v}_K^{+} (t_0) = \lim_{t \rightarrow t_0^+} \frac{\mathbf{x}(t) - \mathbf{x}(t_0)}{t - t_0}.
> \\]

TODO: polish the theorem below.

> **Theorem \[inner-corner-deriv\].** For any cap \\(K\\), \\(\mathbf{v}_K^+ (t)\\) exists for any \\(0 \leq t < \pi / 2\\) and is equal to the following. ^thm-inner-corner-deriv
> \\[
> \begin{align*}
> \mathbf{v}_K^+(t) = -(g_K^+(t) - 1) \cdot u_t + (h_K^+(t) - 1) \cdot v_t
> \end{align*}
> \\]
> Likewise, \\(\mathbf{v}_K^- (t)\\) exists for all \\(0 < t \leq \pi / 2\\) and is equal to the following.
> \\[
> \begin{equation*}
> \mathbf{v}_K^-(t) = -(g_K^-(t) - 1) \cdot u_t + (h_K^-(t) - 1) \cdot v_t
> \end{equation*}
> \\]

*Proof.* (sketch) Take any \\(0 \leq t < \pi / 2\\) and set \\(s = t + \delta\\) for sufficiently small and arbitrary \\(\delta > 0\\). We simplify \\(\mathbf{v}^+(t) = \lim_{\delta \rightarrow 0^+}(\mathbf{x}(s) - \mathbf{x}(t)) / \delta\\).

Since \\(A_{t, s}\\) is on lines \\(a(t)\\) and \\(a(s)\\), it satisfies both \\[A_{t, s} \cdot u_t = \mathbf{x}(t) \cdot u_t + 1\\] and \\[A_{t, s} \cdot u_s = \mathbf{x}(s) \cdot u_s + 1.\\]
Rewrite \\(u_s = \cos \delta \cdot u_t + \sin \delta \cdot v_t\\) on the second equation and we have
\\[
\begin{align*}
	A_{t, s} \cos \delta \cdot u_t + A_{t, s} \sin \delta \cdot v_t =  	\cos \delta (\mathbf{x}(s) \cdot u_t) + \sin \delta (\mathbf{x}(s) \cdot v_t) + 1.
\end{align*}
\\]
Group by \\(\cos \delta\\) and \\(\sin \delta\\) and substitute \\(A_{t, s} \cdot u_t\\) with first equation then
\\[ \cos \delta (\mathbf{x}(s) \cdot u_t - \mathbf{x}(t) \cdot u_t) + (1 - \cos \delta)
	= \sin \delta (A_{t, s}  (s) \cdot v_t - \mathbf{x}(s) \cdot v_t) .
	\\]
Divide by \\(\delta\\) and send \\(\delta\\) to zero. We get
\\[ \mathbf{v}_K^+(t) \cdot u_t  = (A^+(t) - \mathbf{x}(t)) \cdot v_t\\]
Note that \\(g_t^+ = (\mathbf{y}(t) - A^+(t)) \cdot v_t = (\mathbf{x}(t) - A^+(t))\cdot v_t + 1\\) so we have
\\[ \mathbf{v}_K^+(t) \cdot u_t = 1 - g_t ^+.\\]
A similar argument can be applied to show \\(\mathbf{v}^+(t) \cdot v_t = h_t^+ - 1\\) and thus the first equation of the theorem. A symmetric argument shows the second equation of the theorem. â–¡
